Move and update the code of the AVL tree

tests/src/avl/src/avl.rs
@@ -1,0 +1,475 @@
+#![feature(register_tool)]
+#![register_tool(aeneas)]
+#![feature(box_patterns)]
+#![feature(let_chains)]
+
+impl Ord for i32 {
+    fn cmp(&self, other: &Self) -> Ordering {
+        if *self < *other {
+            Ordering::Less
+        } else if *self == *other {
+            Ordering::Equal
+        } else {
+            Ordering::Greater
+        }
+    }
+}
+
+pub enum Ordering {
+    Less,
+    Equal,
+    Greater,
+}
+
+pub trait Ord {
+    fn cmp(&self, other: &Self) -> Ordering;
+}
+
+struct Node<T> {
+    value: T,
+    left: Option<Box<Node<T>>>,
+    right: Option<Box<Node<T>>>,
+    balance_factor: i8,
+}
+
+pub struct Tree<T> {
+    root: Option<Box<Node<T>>>,
+}
+
+impl<T> Node<T> {
+    fn rotate_left(root: &mut Box<Node<T>>, mut z : Box<Node<T>>) {
+        // We do (root is X):
+        //
+        //        X
+        //       /
+        //      A   Z
+        //         / \
+        //        B   C
+        //
+        //        ~>
+        //
+        //        Z
+        //       / \
+        //      X   C
+        //     / \
+        //    A   B
+
+        let b = std::mem::replace(&mut z.left, None);
+        root.right = b;
+        //        X
+        //       / \
+        //      A   B
+        //
+        //        Z
+        //         \
+        //          C
+        
+        let x = std::mem::replace(root, z);
+        root.left = Some(x); // root is now Z
+        //        Z
+        //       / \
+        //      X   C
+        //     / \
+        //    A   B
+
+        // Update the balance factors
+        if let Some(x) = &mut root.left {
+            if root.balance_factor == 0 {
+                x.balance_factor = 1;
+                root.balance_factor = -1;
+            }
+            else {
+                x.balance_factor = 0;
+                root.balance_factor = 0;
+            }
+        }
+    }
+
+    fn rotate_right(root: &mut Box<Node<T>>, mut z : Box<Node<T>>) {
+        // We do (root is X):
+        //
+        //        X
+        //         \
+        //      Z   C
+        //     / \
+        //    A   B
+        //
+        //        ~>
+        //
+        //        Z
+        //       / \
+        //      A   X
+        //         / \
+        //        B   C
+
+        let b = std::mem::replace(&mut z.right, None);
+        root.left = b;
+        //        X
+        //       / \
+        //      B   C
+        //
+        //        Z
+        //       /
+        //      A
+        
+        let x = std::mem::replace(root, z);
+        root.right = Some(x); // root is now Z
+
+        // Update the balance factors
+        if let Some(x) = &mut root.right {
+            if root.balance_factor == 0 {
+                x.balance_factor = -1;
+                root.balance_factor = 1;
+            }
+            else {
+                x.balance_factor = 0;
+                root.balance_factor = 0;
+            }
+        }
+    }
+
+    fn rotate_right_left(root : &mut Box<Node<T>>, mut z : Box<Node<T>>) {
+        // We do (root is X):
+        //
+        //        X
+        //       /
+        //      0   Z
+        //         / \
+        //        Y   1
+        //       / \
+        //      A  B
+        //
+        //        ~>
+        //
+        //          Y
+        //        /   \
+        //      X       Z
+        //     / \     / \
+        //    0   A   B   1
+
+        let mut y = std::mem::replace(&mut z.left, None).unwrap();
+        let a = std::mem::replace(&mut y.left, None);
+        let b = std::mem::replace(&mut y.right, None);
+        z.left = b;
+        root.right = a;
+
+        let x = std::mem::replace(root, y);
+        root.left = Some(x);
+        root.right = Some(z);
+
+        // Update the balance factors
+        if let Some(x) = &mut root.left && let Some(z) = &mut root.right {
+            if root.balance_factor == 0 {
+                x.balance_factor = 0;
+                z.balance_factor = 0;
+            }
+            else if root.balance_factor > 0 {
+                x.balance_factor = -1;
+                z.balance_factor = 0;
+            }
+            else {
+                x.balance_factor = 0;
+                z.balance_factor = 1;
+            }
+            root.balance_factor = 0;
+        }
+        else {
+            panic!();
+        }
+    }
+
+    fn rotate_left_right(root : &mut Box<Node<T>>, mut z : Box<Node<T>>) {
+        // We do (root is X):
+        //
+        //        X
+        //         \
+        //      Z   1
+        //     / \
+        //    0   Y
+        //       / \
+        //      B   A
+        //
+        //        ~>
+        //
+        //          Y
+        //        /   \
+        //      Z       X
+        //     / \     / \
+        //    0   B   A   1
+
+        let mut y = std::mem::replace(&mut z.right, None).unwrap();
+        let a = std::mem::replace(&mut y.right, None);
+        let b = std::mem::replace(&mut y.left, None);
+        z.right = b;
+        root.left = a;
+
+        let x = std::mem::replace(root, y);
+        root.left = Some(z);
+        root.right = Some(x);
+
+        // Update the balance factors
+        if let Some(x) = &mut root.right && let Some(z) = &mut root.left {
+            if root.balance_factor == 0 {
+                x.balance_factor = 0;
+                z.balance_factor = 0;
+            }
+            else if root.balance_factor < 0 {
+                x.balance_factor = 1;
+                z.balance_factor = 0;
+            }
+            else {
+                x.balance_factor = 0;
+                z.balance_factor = -1;
+            }
+            root.balance_factor = 0;
+        }
+        else {
+            panic!();
+        }
+    }
+}
+
+impl<T: Ord> Node<T> {
+    fn insert_in_left(node: &mut Box<Node<T>>, value: T) -> bool {
+        if Tree::insert_in_opt_node(&mut node.left, value) {
+            // We increased the height of the left node
+            node.balance_factor -= 1;
+            if node.balance_factor == -2 {
+                // The node is left-heavy: we need to rebalance
+                let left = std::mem::replace(&mut node.left, Option::None).unwrap();
+                if left.balance_factor <= 0 {
+                    Node::rotate_right(node, left);
+                }
+                else {
+                    Node::rotate_left_right(node, left);
+                }
+                // In order to udnerstand what happens here we need a drawing.
+                // In effect, as we rebalanced the tree, the total height did not
+                // increase compared to before the insertion operation.
+                false
+            }
+            else {
+                // If the balance factor changed from 1 to 0: the height did not
+                // change (we increased the height of the left subtree, which
+                // has now the same height as the right subtree).
+                // If it changed from 0 to -1: the subtrees originally had the same
+                // height and now the left subtree is strictly heigher than the
+                // right subtree: the total height is increased.
+                // This means that the height changed iff the new balance factor
+                // is different from 0
+                node.balance_factor != 0
+            }
+        }
+        else {
+            // The height did not change
+            false
+        }
+    }
+    
+    fn insert_in_right(node: &mut Box<Node<T>>, value: T) -> bool {
+        // Insert in the right sutbree, and check if we increased its height
+        if Tree::insert_in_opt_node(&mut node.right, value) {
+            // We increased the height of the right node
+            node.balance_factor += 1;
+
+            if node.balance_factor == 2 {
+                // The node is right-heavy: we need to rebalance
+                let right = std::mem::replace(&mut node.right, Option::None).unwrap();
+                if right.balance_factor >= 0 {
+                    Node::rotate_left(node, right);
+                }
+                else {
+                    Node::rotate_right_left(node, right);
+                }
+                // In order to udnerstand what happens here we need a drawing.
+                // In effect, as we rebalanced the tree, the total height did not
+                // increase compared to before the insertion operation.
+                false
+            }
+            else {
+                // If the balance factor changed from -1 to 0: the height did not
+                // change (we increased the height of the right subtree, which
+                // has now the same height as the left subtree).
+                // If it changed from 0 to 1: the subtrees originally had the same
+                // height and now the right subtree is strictly heigher than the
+                // left subtree: the total height is increased.
+                // This means that the height changed iff the new balance factor
+                // is different from 0
+                node.balance_factor != 0
+            }
+        }
+        else {
+            // The height of the right subtree did not change so the total
+            // height did not change.
+            false
+        }
+    }
+    
+    // Return [true] if we increased the height of the tree
+    fn insert(node: &mut Box<Node<T>>, value: T) -> bool {
+        let ordering = value.cmp(&(*node).value);
+
+        // Something important: we need to recompute the balance factor
+        // from the current balance factor and the change in height. Also,
+        // we need to compute whether the height of the current tree increased
+        // or not.
+        match ordering {
+            Ordering::Less => {
+                Node::insert_in_left(node, value)
+            },
+            Ordering::Equal => false,
+            Ordering::Greater => {
+                Node::insert_in_right(node, value)
+            }
+        }
+    }
+}
+
+impl<T: Ord> Tree<T> {
+    pub fn new() -> Self {
+        Self { root: None }
+    }
+
+    pub fn find(&self, value: T) -> bool {
+        let mut current_tree = &self.root;
+
+        while let Some(current_node) = current_tree {
+            match current_node.value.cmp(&value) {
+                Ordering::Less => current_tree = &current_node.right,
+                Ordering::Equal => return true,
+                Ordering::Greater => current_tree = &current_node.left,
+            }
+        }
+
+        false
+    }
+
+    fn insert_in_opt_node(node: &mut Option<Box<Node<T>>>, value: T) -> bool {
+        match node {
+            Some(ref mut node) => {
+                Node::insert(node, value)
+            }
+            None => {
+                *node = Some(Box::new(Node {
+                    value,
+                    left: None,
+                    right: None,
+                    balance_factor: 0,
+                }));
+                true
+            }
+        }
+    }
+
+    /// Insert a value and return [true] if the height of the tree increased.
+    pub fn insert(&mut self, value: T) -> bool {
+        Tree::insert_in_opt_node(&mut self.root, value)
+    }
+}
+
+
+#[cfg(test)]
+mod tests {
+    use super::*;
+
+    impl Ord for usize {
+        fn cmp(&self, other: &Self) -> Ordering {
+            if *self < *other {
+                Ordering::Less
+            } else if *self == *other {
+                Ordering::Equal
+            } else {
+                Ordering::Greater
+            }
+        }
+    }
+
+    fn get_max<T: Ord + Copy>(a: T, b: T) -> T {
+        match a.cmp(&b) {
+            Ordering::Less => b,
+            Ordering::Equal => b,
+            Ordering::Greater => a,
+        }
+    }
+
+
+    impl<T> Node<T> {
+        fn height(&self) -> usize {
+            1 + get_max(self.right.as_deref().map_or(0, |n| n.height()), self.left.as_deref().map_or(0, |n| n.height()))
+        }
+
+        fn balance_factor(&self) -> isize {
+            self.right.as_deref().map_or(0, |n| n.height()) as isize - self.left.as_deref().map_or(0, |n| n.height()) as isize
+        }
+
+        fn check_inv(&self) {
+            let bf = self.balance_factor();
+            assert!(-1 <= bf && bf <= 1);
+            assert!(bf == self.balance_factor as isize);
+            if let Some(n) = &self.left {
+                n.check_inv();
+            }
+            if let Some(n) = &self.right {
+                n.check_inv();
+            }
+        }
+    }
+
+    impl<T> Tree<T> {
+        fn check_inv(&self) {
+            if let Some(n) = &self.root {
+                n.check_inv();
+            }
+        }
+    }
+
+    #[test]
+    fn test1() {
+        let mut t : Tree<i32> = Tree::new();
+
+        // Always inserting to the right
+        for i in 0..100 {
+            t.insert(i);
+            t.check_inv();
+        }
+    }
+
+    #[test]
+    fn test2() {
+        let mut t : Tree<i32> = Tree::new();
+
+        // Always inserting to the left
+        for i in 0..(-100) {
+            t.insert(i);
+            t.check_inv();
+        }
+    }
+
+    #[test]
+    fn test3() {
+        let mut t : Tree<i32> = Tree::new();
+
+        // Always inserting to the right
+        for i in 0..100 {
+            t.insert(i);
+            t.check_inv();
+        }
+
+        // Always inserting to the left
+        for i in 0..(-100) {
+            t.insert(i);
+            t.check_inv();
+        }
+    }
+
+    #[test]
+    fn test4() {
+        let mut t : Tree<i32> = Tree::new();
+
+        // Simulating randomness here
+        for i in 0..100 {
+            t.insert((i * i + 23 * i) % 17);
+            t.check_inv();
+        }
+    }
+}
